@prefix : <http://lari-datasets.ilc.cnr.it/lemonBib#> .
@prefix cito: <http://purl.org/spar/cito/> .
@prefix dct: <http://purl.org/dc/terms/> .
@prefix lexinfo: <http://www.lexinfo.net/ontology/2.0/lexinfo#> .
@prefix ontolex: <http://www.w3.org/ns/lemon/ontolex#> .
@prefix owl: <http://www.w3.org/2002/07/owl#> .
@prefix rdf: <http://www.w3.org/1999/02/22-rdf-syntax-ns#> .
@prefix rdfs: <http://www.w3.org/2000/01/rdf-schema#> .
@prefix xml: <http://www.w3.org/XML/1998/namespace> .
@prefix xsd: <http://www.w3.org/2001/XMLSchema#> .

:Attestation a rdfs:Class ;
    rdfs:label "Attestation"@en ;
    rdfs:comment "'Attestation' is a class that consists of individuals that reifies the relationship of lexical attestation between an element in a lexicon and a bibliographic element"@en .

<http://lari-datasets.ilc.cnr.it/lemonBib#> a owl:Ontology ;
    dct:contributor <http://www.ilc.cnr.it/en/content/anas_fahad_khan> ;
    dct:description "lemonBib is an extension of the ontolex-lemon model that provides concepts and properties that are useful in representing lexical attestations."@en ;
    dct:issued "2018-05-24" ;
    dct:rights "CC-BY" ;
    dct:title "lemonBib"@en ;
    owl:imports <http://www.w3.org/ns/lemon/all>,
        <http://www.w3.org/ns/lemon/ontolex> ;
    owl:versionInfo "Version 0.1.0" .

:attestationCitation a rdf:Property,
        owl:ObjectProperty ;
    rdfs:label "attestation citation"@en ;
    rdfs:comment "'attestationCitation' is an object property that relates an Attestation with a citation."@en ;
    rdfs:domain :Attestation .

:attests a rdf:Property,
        owl:ObjectProperty ;
    rdfs:label "attests"@en ;
    rdfs:comment "'isAttestedBy' is an object property that relates an individual of the class with a lexical element."@en ;
    rdfs:domain :Attestation .

:conjectural a rdf:Property,
        owl:DatatypeProperty ;
    rdfs:label "conjectural"@en ;
    rdfs:comment "'conjectural' is a datatype property that relates an Attestation with a boolean value that specifies if it refers to a conjectural text or not."@en ;
    rdfs:domain :Attestation ;
    rdfs:range xsd:boolean .

:foundIn a rdf:Property,
        owl:ObjectProperty ;
    rdfs:label "found in"@en ;
    rdfs:comment "'foundIn' is an object property that relates an Attestation with a location in a text where it can be found."@en ;
    rdfs:domain :Attestation .

:hasBiblScope a rdf:Property,
        owl:DatatypeProperty ;
    rdfs:label "has bibliographic scope"@en ;
    rdfs:comment "'hasBiblScope' is a datatype property that relates a bibliographic entity with specific bibliographic information."@en .

:hasContext a rdf:Property,
        owl:DatatypeProperty ;
    rdfs:label "has context"@en ;
    rdfs:comment "'hasContext' is a datatype property that relates an Attestation with a string."@en ;
    rdfs:domain :Attestation ;
    rdfs:range xsd:string .

:hasURN a rdf:Property,
        owl:DatatypeProperty ;
    rdfs:label "has URN"@en ;
    rdfs:comment "'hasURN' is a datatype property that relates a bibliographic entity with a string URN."@en .

:involvedinAttestation a rdf:Property,
        owl:ObjectProperty ;
    rdfs:label "involved in attesation"@en ;
    rdfs:comment "'involvedinAttestation' is an object property that relates a citation with an Attestation."@en ;
    rdfs:range :Attestation .

:isAttestedBy a rdf:Property,
        owl:ObjectProperty ;
    rdfs:label "is attested by"@en ;
    rdfs:comment "'isAttestedBy' is an object property that relates a lexical element with an individual of the class Attestation."@en ;
    rdfs:range :Attestation .

